sub proj inversion

src/assoc.v
@@ -19,13 +19,6 @@ Definition assoc (g: tctx) (gt:gtt) :=
         issubProj Tp gt p) /\
          ~ isgPartsC p gt -> forall Tpx, M.find p g = Some Tpx -> Tpx=ltt_end.
 
-Definition send_cond (xs:list (option (sort*ltt))) (ys:list (option (sort*gtt))) (p:part) := 
-    Forall2R (fun x y => x=None 
-        \/ (exists s elx s' ely, y=Some (s',ely)/\ x=Some (s,elx) /\ 
-        subsort s s' /\
-        issubProj elx ely p)) xs ys.
-Check send_cond.
-
 Lemma subtype_end_inv : forall t, subtypeC t ltt_end -> t=ltt_end.
 Proof.
     intros.
@@ -33,9 +26,7 @@ Proof.
     pinversion H;apply subtype_monotone.
 Qed.
 
-Definition send_cond2 (t:ltt) (ys:list(option(sort*gtt))) (p:part) :=
-    Forall (fun y=> (y=None)\/ 
-    (exists s' Gy, y=Some (s', Gy) /\issubProj t Gy p)) ys.
+
 
 Lemma subtype_send_inv1 : forall q xs T, 
 subtypeC (ltt_send q xs) T -> exists ys, T=ltt_send q ys.
@@ -71,10 +62,7 @@ Inductive context_height: gtth -> nat -> Prop :=
         SList hs -> Forall (fun u=> u=None \/ 
             (exists s h, u=Some (s,h) /\ context_height h x)) hs->
         context_height (gtth_send p q hs) (S x).
-        
-Section height_induction.
-    
-End height_induction.
+
 
 Lemma subtype_recv_inv1 : forall q xs T, 
 subtypeC (ltt_recv q xs) T -> exists ys, T=ltt_recv q ys.
@@ -155,9 +143,24 @@ projectionC g p (ltt_send q xs) -> isgPartsC p g.
 Proof.
     intros. pinversion H;subst;crush. apply proj_mon.
 Qed.
-Lemma empty_not_wfg_proj: forall p q g, wfgC g -> projectionC g p (ltt_send q []) -> False.
-Proof. 
-Admitted.
+Section subproj_inversion.
+Definition send_cond (xs:list (option (sort*ltt))) (ys:list (option (sort*gtt))) (p:part) := 
+    Forall2R (fun x y => x=None 
+        \/ (exists s elx s' ely, y=Some (s',ely)/\ x=Some (s,elx) /\ 
+        subsort s s' /\
+        issubProj elx ely p)) xs ys.
+
+Definition subproj_cont_cond (t:ltt) (ys:list(option(sort*gtt))) (p:part) :=
+    Forall (fun y=> (y=None)\/ 
+    (exists s' Gy, y=Some (s', Gy) /\issubProj t Gy p)) ys.
+
+Definition recv_cond (xs:list (option (sort*ltt))) (ys:list (option (sort*gtt))) (p:part) := 
+    Forall2R (fun y x => y=None 
+        \/ (exists s elx s' ely, y=Some (s',ely)/\ x=Some (s,elx) /\ 
+        subsort s' s /\
+        issubProj elx ely p)) ys xs.
+
+
 Lemma subproj_helper: forall xs ys gs p,  Forall2R
 (fun u v : option (sort * ltt) =>
 u = None \/
@@ -185,23 +188,62 @@ Proof.
     exists x2, x4, x3,x0. unfold issubProj. crush. exists x5. destruct H5;crush.
     inversion H;inversion H0;subst. eapply IHxs with (gs:=gs) (ys:=ys);crush.
 Qed.
-Check M.merge.
-
+Lemma subproj_helper2:  forall gs p q xs x0  ys, SList xs -> 
+subtypeC (ltt_send q xs) (ltt_send q x0) ->
+(isMerge (ltt_send q x0) ys \/ ys= [] )->
+Forall2R
+(fun u v : option (sort * ltt) =>
+u = None \/
+(exists (s s' : sort) (t t' : ltt),
+u = Some (s, t) /\ v = Some (s', t') /\
+subsort s s' /\ subtypeC t t')) xs x0 ->
+Forall2
+(fun (u : option (sort * gtt)) (v : option ltt) =>
+u = None /\ v = None \/
+(exists (s : sort) (g : gtt) (t : ltt),
+u = Some (s, g) /\ v = Some t /\ upaco3 projection bot3 g p t)) gs
+ys ->
+Forall
+(fun y : option (sort * gtt) =>
+y = None \/
+(exists (s' : sort) (Gy : gtt),
+y = Some (s', Gy) /\
+(exists tg : ltt, projectionC Gy p tg /\ subtypeC (ltt_send q xs) tg)))
+gs.
+Proof.
+    induction gs. crush.
+    intros.
+    destruct ys. inversion H3.
+    constructor. 
+    {
+        inversion H3;subst.
+        destruct a;crush.
+        right. exists x,x1. crush.
+        exists (ltt_send q x0).
+        inversion H4;subst;
+        destruct H7;crush. 
+    }
+    {
+        eapply IHgs with (x0:=x0) (ys:=ys);crush.
+        inversion H4;crush.
+        
+        inversion H3;crush.
+    }        
+Qed.
 Lemma subproj_inv_send: forall q xs p G, wfgC G -> 
     SList xs -> issubProj (ltt_send q xs) G p -> 
     (exists ys, G=gtt_send p q ys /\ send_cond xs ys p)
     \/ (exists s t ys, G=gtt_send s t ys /\ p <> s /\ p<> t /\ 
-        send_cond2 (ltt_send q xs) ys p ).
+        subproj_cont_cond (ltt_send q xs) ys p ).
 Proof.
     intros.
     unfold issubProj in H1.
     destr_hyps.
-    
+    pose proof H2 as Hsubpr.
     apply subtype_send_strong_inv in H2.
     destruct H2. destruct H2. subst.
     rename H3 into Hsubtpcond.
     (*ltt_send q x0 is the supertype*)
-    Print projection.
     pinversion H1; try apply proj_mon; subst.
     {
         
@@ -215,13 +257,117 @@ Proof.
             | [H:Forall2 _  [] (?a::?b)  |- _] => inversion H 
             | [H:wfgC (gtt_send _ _ []) |- _] => apply empty_not_wfg in H end);
         crush.
-        eapply subproj_helper with(ys:=o1::x0);crush.
+        apply subproj_helper with(ys:=o1::x0);crush.
     }
     {
-
-        right. exists p0,q0,xs0. unfold send_cond2. crush. 
+        right. exists p0,q0,xs0. unfold subproj_cont_cond. crush. 
         unfold issubProj.
-        (*ys: list that merges to ltt_send q x0*)
-        inversion H1;subst. crush.
+        destruct ys. inversion H7.
+        eapply subproj_helper2 with (x0:=x0) (ys:=o::ys);crush.
     }
 Qed.
+
+Lemma subproj_helper_recv: forall xs ys gs p,
+Forall2R (fun u v => 
+(u = None) \/ (exists s s' t t', u = Some(s,t) /\ 
+v = Some (s',t') /\ subsort s s' /\ subtypeC t' t)) ys xs
+-> Forall2
+(fun (u : option (sort * gtt)) (v : option (sort * ltt)) =>
+u = None /\ v = None \/
+(exists (s : sort) (g : gtt) (t : ltt),
+u = Some (s, g) /\
+v = Some (s, t) /\ upaco3 projection bot3 g p t))
+gs ys -> Forall2R
+(fun  (y : option (sort * gtt)) (x : option (sort * ltt)) =>
+y = None \/
+(exists (s : sort) (elx : ltt) (s' : sort) (ely : gtt),
+y = Some (s', ely) /\
+x = Some (s, elx) /\ subsort s' s /\ issubProj elx ely p)) gs xs.
+Proof.
+    intros xs.
+    induction xs; intros; destruct ys;
+    destruct gs;try invalid_forall_wfg;crush. constructor. constructor.
+    constructor. destruct o0;crush. right. 
+    inversion H. inversion H0. destruct H4;destruct H10;crush.
+    exists x3,x5,x2,x0. unfold issubProj. crush. exists x4. destruct H5;crush.
+
+    inversion H;inversion H0;subst. eapply IHxs with (gs:=gs)(ys:=ys);crush.
+Qed.
+
+Lemma subproj_helper_2_recv:  forall gs p q xs x0  ys, SList xs -> 
+subtypeC (ltt_recv q xs) (ltt_recv q x0) ->
+(isMerge (ltt_recv q x0) ys \/ ys= [] )->
+Forall2R (fun u v => (u = None) \/ 
+(exists s s' t t', u = Some(s,t) /\ v = Some (s',t') /\ 
+subsort s s' /\ subtypeC t' t)) x0 xs ->
+Forall2
+(fun (u : option (sort * gtt)) (v : option ltt) =>
+u = None /\ v = None \/
+(exists (s : sort) (g : gtt) (t : ltt),
+u = Some (s, g) /\ v = Some t /\ upaco3 projection bot3 g p t)) gs
+ys ->
+Forall
+(fun y : option (sort * gtt) =>
+y = None \/
+(exists (s' : sort) (Gy : gtt),
+y = Some (s', Gy) /\
+(exists tg : ltt, projectionC Gy p tg /\ subtypeC (ltt_recv q xs) tg)))
+gs.
+Proof.
+    induction gs. crush.
+    intros.
+    destruct ys. inversion H3.
+    constructor. 
+    {
+        inversion H3;subst.
+        destruct a;crush.
+        right. exists x,x1. crush.
+        exists (ltt_recv q x0).
+        inversion H4;subst;
+        destruct H7;crush. 
+    }
+    {
+        eapply IHgs with (x0:=x0) (ys:=ys);crush.
+        inversion H4;crush.
+        
+        inversion H3;crush.
+    }        
+Qed.
+
+Lemma subproj_inv_recv: forall q xs p G, wfgC G -> 
+    SList xs -> issubProj (ltt_recv q xs) G p -> 
+    (exists ys, G=gtt_send q p ys /\ recv_cond xs ys p)
+    \/ (exists s t ys, G=gtt_send s t ys /\ p <> s /\ p<> t /\ 
+        subproj_cont_cond (ltt_recv q xs) ys p ).
+Proof.
+    intros.
+    unfold issubProj in H1.
+    destr_hyps.
+    pose proof H2 as Hsubpr.
+    apply subtype_recv_strong_inv in H2.
+    destruct H2. destruct H2. subst.
+    rename H3 into Hsubtpcond.
+    pinversion H1; try apply proj_mon; subst.
+    {
+        
+        (*G=gtt_send r q xs0*)
+        rename H8 into Hprojcond.
+        left. exists xs0. split; try reflexivity. subst.
+        unfold send_cond.
+        destruct xs; destruct xs0;crush;destruct x0;
+        try (match goal with | 
+            [H:Forall2 _  (?a::?b) [] |- _] => inversion H 
+            | [H:Forall2 _  [] (?a::?b)  |- _] => inversion H 
+            | [H:wfgC (gtt_send _ _ []) |- _] => apply empty_not_wfg in H end);
+        crush.
+        unfold recv_cond.
+        apply subproj_helper_recv with(ys:=o1::x0);crush.
+    }
+    {
+        right. exists p0,q0,xs0. unfold subproj_cont_cond. crush. 
+        unfold issubProj.
+        destruct ys. inversion H7.
+        eapply subproj_helper_2_recv with (x0:=x0) (ys:=o::ys);crush.
+    }
+Qed.
+End subproj_inversion.
