src/local.v
@@ -387,7 +387,8 @@ Proof.
   apply subtype_monotone.
 Qed.
 
-Lemma subtype_recv_inv : forall pt xs ys, subtypeC (ltt_recv pt xs) (ltt_recv pt ys) -> Forall2R (fun u v => (u = None) \/ (exists s s' t t', u = Some(s,t) /\ v = Some (s',t') /\ subsort s s' /\ subtypeC t' t)) ys xs.
+Lemma subtype_recv_inv : forall pt xs ys, subtypeC (ltt_recv pt xs) (ltt_recv pt ys) -> 
+  Forall2R (fun u v => (u = None) \/ (exists s s' t t', u = Some(s,t) /\ v = Some (s',t') /\ subsort s s' /\ subtypeC t' t)) ys xs.
 Proof.
   intros pt xs ys. revert pt xs.
   induction ys; intros. constructor.
